simplify proof of rsapss

code/rsapss/Hacl.Impl.RSAPSS.fst
@@ -14,12 +14,14 @@ module ST = FStar.HyperStack.ST
 module Hash = Spec.Agile.Hash
 module SB = Hacl.Spec.Bignum
 module BB = Hacl.Spec.Bignum.Base
+module SD = Hacl.Spec.Bignum.Definitions
 module BN = Hacl.Bignum
 module BE = Hacl.Bignum.Exponentiation
 module BM = Hacl.Bignum.Montgomery
 
 module S = Spec.RSAPSS
 module LS = Hacl.Spec.RSAPSS
+module LSeq = Lib.Sequence
 
 module RP = Hacl.Impl.RSAPSS.Padding
 module RM = Hacl.Impl.RSAPSS.MGF
@@ -28,7 +30,7 @@ module RK = Hacl.Impl.RSAPSS.Keys
 #reset-options "--z3rlimit 150 --fuel 0 --ifuel 0"
 
 inline_for_extraction noextract
-let modBits_t (t:limb_t) = modBits:size_t{0 < v modBits /\ 128 * v (blocks modBits (size (bits t))) <= max_size_t}
+let modBits_t (t:limb_t) = modBits:size_t{1 < v modBits /\ 128 * SD.blocks (v modBits) (bits t) <= max_size_t}
 
 
 inline_for_extraction noextract
@@ -52,10 +54,10 @@ let rsapss_sign_bn_st (t:limb_t) (ke:BE.exp t) (modBits:modBits_t t) =
 inline_for_extraction noextract
 val rsapss_sign_bn: #t:limb_t -> ke:BE.exp t -> modBits:modBits_t t -> rsapss_sign_bn_st t ke modBits
 let rsapss_sign_bn #t ke modBits eBits dBits skey m m' s =
-  [@inline_let] let bits = size (bits t) in
-  let nLen = blocks modBits bits in
-  let eLen = blocks eBits bits in
-  let dLen = blocks dBits bits in
+  [@inline_let] let bits : size_pos = bits t in
+  let nLen = blocks modBits (size bits) in
+  let eLen = blocks eBits (size bits) in
+  let dLen = blocks dBits (size bits) in
 
   let n  = sub skey 0ul nLen in
   let r2 = sub skey nLen nLen in
@@ -67,6 +69,100 @@ let rsapss_sign_bn #t ke modBits eBits dBits skey m m' s =
   let eq_m = BN.bn_eq_mask nLen m m' in
   mapT nLen s (logand eq_m) s;
   BB.unsafe_bool_of_limb eq_m
+
+
+inline_for_extraction noextract
+let rsapss_sign_msg_to_bn_st (t:limb_t) (a:Hash.algorithm{S.hash_is_supported a}) (modBits:modBits_t t) =
+  let len = blocks modBits (size (bits t)) in
+    sLen:size_t
+  -> salt:lbuffer uint8 sLen
+  -> msgLen:size_t
+  -> msg:lbuffer uint8 msgLen
+  -> m:lbignum t len ->
+  Stack unit
+  (requires fun h ->
+    live h salt /\ live h msg /\ live h m /\
+    disjoint salt msg /\ disjoint m msg /\ disjoint m salt /\
+    as_seq h m == LSeq.create (v len) (uint #t 0) /\
+    LS.rsapss_sign_pre a (v modBits) (v sLen) (as_seq h salt) (v msgLen) (as_seq h msg))
+  (ensures  fun h0 _ h1 -> modifies (loc m) h0 h1 /\
+    as_seq h1 m == LS.rsapss_sign_msg_to_bn a (v modBits) (v sLen) (as_seq h0 salt) (v msgLen) (as_seq h0 msg))
+
+
+inline_for_extraction noextract
+val rsapss_sign_msg_to_bn:
+    #t:limb_t
+  -> a:Hash.algorithm{S.hash_is_supported a}
+  -> modBits:modBits_t t ->
+  rsapss_sign_msg_to_bn_st t a modBits
+
+let rsapss_sign_msg_to_bn #t a modBits sLen salt msgLen msg m =
+  push_frame ();
+  [@inline_let] let bits : size_pos = bits t in
+  [@inline_let] let numb : size_pos = numbytes t in
+  let nLen = blocks modBits (size bits) in
+
+  let emBits = modBits -! 1ul in
+  let emLen = blocks emBits 8ul in
+  [@inline_let] let mLen = blocks emLen (size numb) in
+
+  let em = create emLen (u8 0) in
+  RP.pss_encode a sLen salt msgLen msg emBits em;
+  LS.blocks_bits_lemma t (v emBits);
+  LS.blocks_numb_lemma t (v emBits);
+  assert (SD.blocks (v emBits) bits = v mLen);
+  assert (numb * v mLen <= max_size_t);
+  assert (v mLen <= v nLen);
+
+  let h' = ST.get () in
+  update_sub_f h' m 0ul mLen
+    (fun h -> SB.bn_from_bytes_be (v emLen) (as_seq h' em))
+    (fun _ -> BN.bn_from_bytes_be emLen em (sub m 0ul mLen));
+  pop_frame ()
+
+
+inline_for_extraction noextract
+let rsapss_sign_compute_sgnt_st (t:limb_t) (ke:BE.exp t) (a:Hash.algorithm{S.hash_is_supported a}) (modBits:modBits_t t) =
+  let len = blocks modBits (size (bits t)) in
+    eBits:size_t
+  -> dBits:size_t{LS.skey_len_pre t (v modBits) (v eBits) (v dBits)}
+  -> skey:lbignum t (2ul *! len +! blocks eBits (size (bits t)) +! blocks dBits (size (bits t)))
+  -> m:lbignum t len
+  -> sgnt:lbuffer uint8 (blocks modBits 8ul) ->
+  Stack bool
+  (requires fun h -> len == ke.BE.mont.BM.bn.BN.len /\
+    live h sgnt /\ live h skey /\ live h m /\
+    disjoint sgnt skey /\ disjoint m sgnt /\ disjoint m skey)
+  (ensures  fun h0 eq_m h1 -> modifies (loc sgnt) h0 h1 /\
+    (eq_m, as_seq h1 sgnt) == LS.rsapss_sign_compute_sgnt a (v modBits) (v eBits) (v dBits) (as_seq h0 skey) (as_seq h0 m))
+
+
+inline_for_extraction noextract
+val rsapss_sign_compute_sgnt:
+    #t:limb_t
+  -> ke:BE.exp t
+  -> a:Hash.algorithm{S.hash_is_supported a}
+  -> modBits:modBits_t t ->
+  rsapss_sign_compute_sgnt_st t ke a modBits
+
+let rsapss_sign_compute_sgnt #t ke a modBits eBits dBits skey m sgnt =
+  push_frame ();
+  let h_init = ST.get () in
+  [@inline_let] let bits : size_pos = bits t in
+  [@inline_let] let numb : size_pos = numbytes t in
+  let nLen = blocks modBits (size bits) in
+
+  let k = blocks modBits 8ul in
+  let s = create nLen (uint #t 0) in
+  let m' = create nLen (uint #t 0) in
+  let eq_b = rsapss_sign_bn ke modBits eBits dBits skey m m' s in
+  LS.blocks_bits_lemma t (v modBits);
+  LS.blocks_numb_lemma t (v modBits);
+  assert (SD.blocks (v k) numb == v nLen);
+  assert (numb * v nLen <= max_size_t);
+  BN.bn_to_bytes_be k s sgnt;
+  pop_frame ();
+  eq_b
 
 
 inline_for_extraction noextract
@@ -102,37 +198,11 @@ val rsapss_sign_:
 
 let rsapss_sign_ #t ke a modBits eBits dBits skey sLen salt msgLen msg sgnt =
   push_frame ();
-  let h_init = ST.get () in
-  [@inline_let] let bits = size (bits t) in
-  [@inline_let] let numb = size (numbytes t) in
-  let nLen = blocks modBits bits in
-
-  let k = blocks modBits 8ul in
-  let emBits = modBits -! 1ul in
-  let emLen = blocks emBits 8ul in
-
-  let em = create emLen (u8 0) in
-  let m  = create nLen (uint #t 0) in
-  let m' = create nLen (uint #t 0) in
-  let s  = create nLen (uint #t 0) in
-
-  RP.pss_encode a sLen salt msgLen msg emBits em;
-  LS.blocks_bits_lemma t (v emBits);
-  LS.blocks_numb_lemma t (v emBits);
-  assert (v (blocks emLen numb) == v (blocks emBits bits));
-  assert (v numb * v (blocks emLen numb) <= max_size_t);
-
-  let h' = ST.get () in
-  update_sub_f h' m 0ul (blocks emLen numb)
-    (fun h -> SB.bn_from_bytes_be (v emLen) (as_seq h' em))
-    (fun _ -> BN.bn_from_bytes_be emLen em (sub m 0ul (blocks emLen numb)));
-
-  let eq_b = rsapss_sign_bn ke modBits eBits dBits skey m m' s in
-  LS.blocks_bits_lemma t (v modBits);
-  LS.blocks_numb_lemma t (v modBits);
-  assert (v (blocks k numb) == v nLen);
-  assert (v numb * v (blocks k numb) <= max_size_t);
-  BN.bn_to_bytes_be k s sgnt;
+  [@inline_let] let bits : size_pos = bits t in
+  let nLen = blocks modBits (size bits) in
+  let m = create nLen (uint #t 0) in
+  rsapss_sign_msg_to_bn a modBits sLen salt msgLen msg m;
+  let eq_b = rsapss_sign_compute_sgnt ke a modBits eBits dBits skey m sgnt in
   pop_frame ();
   eq_b
 
@@ -239,6 +309,95 @@ let rsapss_verify_bn #t ke modBits eBits pkey m_def s =
 
 
 inline_for_extraction noextract
+let rsapss_verify_bn_to_msg_st (t:limb_t) (a:Hash.algorithm{S.hash_is_supported a}) (modBits:modBits_t t) =
+    sLen:size_t
+  -> msgLen:size_t
+  -> msg:lbuffer uint8 msgLen
+  -> m:lbignum t (blocks modBits (size (bits t))) ->
+  Stack bool
+  (requires fun h ->
+    live h msg /\ live h m /\ disjoint m msg /\
+
+    LS.rsapss_verify_pre a (v sLen) (v msgLen) (as_seq h msg))
+  (ensures  fun h0 r h1 -> modifies0 h0 h1 /\
+    r == LS.rsapss_verify_bn_to_msg a (v modBits) (v sLen) (v msgLen) (as_seq h0 msg) (as_seq h0 m))
+
+
+inline_for_extraction noextract
+val rsapss_verify_bn_to_msg:
+    #t:limb_t
+  -> a:Hash.algorithm{S.hash_is_supported a}
+  -> modBits:modBits_t t ->
+  rsapss_verify_bn_to_msg_st t a modBits
+
+let rsapss_verify_bn_to_msg #t a modBits sLen msgLen msg m =
+  push_frame ();
+  [@inline_let] let bits : size_pos = bits t in
+  [@inline_let] let numb : size_pos = numbytes t in
+  let nLen = blocks modBits (size bits) in
+
+  let emBits = modBits -! 1ul in
+  let emLen = blocks emBits 8ul in
+  [@inline_let] let mLen = blocks emLen (size numb) in
+  let em = create emLen (u8 0) in
+
+  LS.blocks_bits_lemma t (v emBits);
+  LS.blocks_numb_lemma t (v emBits);
+  assert (SD.blocks (v emBits) bits == v mLen);
+  assert (numb * v mLen <= max_size_t);
+  assert (v mLen <= v nLen);
+
+  let m1 = sub m 0ul mLen in
+  BN.bn_to_bytes_be emLen m1 em;
+  let res = RP.pss_verify a sLen msgLen msg emBits em in
+  pop_frame ();
+  res
+
+
+inline_for_extraction noextract
+let rsapss_verify_compute_msg_st (t:limb_t) (ke:BE.exp t) (a:Hash.algorithm{S.hash_is_supported a}) (modBits:modBits_t t) =
+   let len = blocks modBits (size (bits t)) in
+    eBits:size_t{LS.pkey_len_pre t (v modBits) (v eBits)}
+  -> pkey:lbignum t (2ul *! len +! blocks eBits (size (bits t)))
+  -> sgnt:lbuffer uint8 (blocks modBits 8ul)
+  -> m:lbignum t len ->
+  Stack bool
+  (requires fun h -> len == ke.BE.mont.BM.bn.BN.len /\
+    live h sgnt /\ live h pkey /\ live h m /\
+    disjoint m sgnt /\ disjoint m pkey /\
+    as_seq h m == LSeq.create (v len) (uint #t 0))
+  (ensures  fun h0 r h1 -> modifies (loc m) h0 h1 /\
+    (r, as_seq h1 m) == LS.rsapss_verify_compute_msg a (v modBits) (v eBits) (as_seq h0 pkey) (as_seq h0 sgnt))
+
+
+inline_for_extraction noextract
+val rsapss_verify_compute_msg:
+    #t:limb_t
+  -> ke:BE.exp t
+  -> a:Hash.algorithm{S.hash_is_supported a}
+  -> modBits:modBits_t t ->
+  rsapss_verify_compute_msg_st t ke a modBits
+
+let rsapss_verify_compute_msg #t ke a modBits eBits pkey sgnt m =
+  push_frame ();
+  [@inline_let] let bits : size_pos = bits t in
+  [@inline_let] let numb : size_pos = numbytes t in
+  let nLen = blocks modBits (size bits) in
+  let k = blocks modBits 8ul in
+
+  let s = create nLen (uint #t 0) in
+  LS.blocks_bits_lemma t (v modBits);
+  LS.blocks_numb_lemma t (v modBits);
+  assert (SD.blocks (v k) numb == v nLen);
+  assert (numb * v nLen <= max_size_t);
+  BN.bn_from_bytes_be k sgnt s;
+
+  let b = rsapss_verify_bn #t ke modBits eBits pkey m s in
+  pop_frame ();
+  b
+
+
+inline_for_extraction noextract
 let rsapss_verify_st1 (t:limb_t) (ke:BE.exp t) (a:Hash.algorithm{S.hash_is_supported a}) (modBits:modBits_t t) =
    let len = blocks modBits (size (bits t)) in
     eBits:size_t{LS.pkey_len_pre t (v modBits) (v eBits)}
@@ -268,35 +427,11 @@ val rsapss_verify_:
 
 let rsapss_verify_ #t ke a modBits eBits pkey sLen sgnt msgLen msg =
   push_frame ();
-  [@inline_let] let bits = size (bits t) in
-  [@inline_let] let numb = size (numbytes t) in
-
-  let nLen = blocks modBits bits in
-  let k = blocks modBits 8ul in
-  let emBits = modBits -! 1ul in
-  let emLen = blocks emBits 8ul in
-
-  let em = create emLen (u8 0) in
+  [@inline_let] let bits : size_pos = bits t in
+  let nLen = blocks modBits (size bits) in
   let m = create nLen (uint #t 0) in
-  let s = create nLen (uint #t 0) in
-  LS.blocks_bits_lemma t (v modBits);
-  LS.blocks_numb_lemma t (v modBits);
-  assert (v (blocks k numb) == v nLen);
-  assert (v numb * v (blocks k numb) <= max_size_t);
-  BN.bn_from_bytes_be k sgnt s;
-
-  let b = rsapss_verify_bn #t ke modBits eBits pkey m s in
-  let res =
-    if b then begin
-      LS.blocks_bits_lemma t (v emBits);
-      LS.blocks_numb_lemma t (v emBits);
-      assert (v (blocks emLen numb) == v (blocks emBits bits));
-      assert (v numb * v (blocks emLen numb) <= max_size_t);
-
-      let m1 = sub m 0ul (blocks emLen numb) in
-      BN.bn_to_bytes_be emLen m1 em;
-      RP.pss_verify a sLen msgLen msg emBits em end
-    else false in
+  let b = rsapss_verify_compute_msg ke a modBits eBits pkey sgnt m in
+  let res = if b then rsapss_verify_bn_to_msg a modBits sLen msgLen msg m else false in
   pop_frame ();
   res
 
